src/OneDisk/OneDiskAPI.v
@@ -31,8 +31,6 @@ Definition diskSize_spec : Specification _ nat unit State :=
       state' = state
   |}.
 
-Definition wipe (state state' : State) := state' = state.
-
 
 Module Type OneDiskAPI.
 
@@ -47,7 +45,7 @@ Module Type OneDiskAPI.
   Axiom read_ok : forall a, prog_spec (read_spec a) (read a) recover abstr.
   Axiom write_ok : forall a v, prog_spec (write_spec a v) (write a v) recover abstr.
   Axiom diskSize_ok : prog_spec diskSize_spec diskSize recover abstr.
-  Axiom recover_noop : rec_noop recover abstr wipe.
+  Axiom recover_noop : rec_noop recover abstr (@no_wipe _).
 
   Hint Resolve read_ok.
   Hint Resolve write_ok.
