src/BadSectorDisk/BadSectorImpl.v
@@ -19,7 +19,7 @@ Module BadSectorDisk <: BadSectorAPI.
   Axiom write_ok : forall a v, prog_spec (write_spec a v) (write a v) recover abstr.
   Axiom getBadSector_ok : prog_spec getBadSector_spec getBadSector recover abstr.
   Axiom diskSize_ok : prog_spec diskSize_spec diskSize recover abstr.
-  Axiom recover_noop : rec_noop recover abstr wipe.
+  Axiom recover_noop : rec_noop recover abstr (@no_wipe _).
 
 End BadSectorDisk.
 
